src/Analysis/Instances/Sign/Sign_Exec.thy
@@ -80,6 +80,17 @@ lemma fun_of_st_cinit_sign_st:
    (\<lambda>x. if is_global x then SZero else STop)"
   by (rule ext) simp
 
+lemma lookup_cinit_sign_st_for [simp]:
+  "fun_of_resolved_st_q_for gs cinit_sign_st x =
+   (if gs x then SZero else STop)"
+  unfolding fun_of_resolved_st_q_for_def
+  by transfer (auto simp: location_of_def split: if_splits)
+
+lemma fun_of_st_cinit_sign_st_for:
+  "fun_of_resolved_st_q_for gs cinit_sign_st =
+   (\<lambda>x. if gs x then SZero else STop)"
+  by (rule ext) simp
+
 theorem sign_tf_st_commute:
   "fun_of_resolved_st_q_for is_global (sign_tf_st a s) =
    apply_tf sign_tf a (fun_of_resolved_st_q_for is_global s)"
@@ -149,6 +160,100 @@ lemma sign_etf_st_exists_unit:
 value "fun_of_resolved_st_q_for is_global top_sign_st ''x''"
 value "fun_of_resolved_st_q_for is_global cinit_sign_st ''Gx''"
 value "fun_of_resolved_st_q_for is_global cinit_sign_st ''x''"
+
+subsection \<open>Classifier-parametric executable transfer\<close>
+
+text \<open>The executable mirror of \<open>sign_tf_for\<close>/\<open>enter_sign_for\<close>, parametric in
+  the classifier, following the same pattern as \<open>ivl_tf_st_for\<close>/
+  \<open>ivl_enter_st_for\<close> for the interval domain.\<close>
+
+definition assume_sign_st_for ::
+  "(vname => bool) => bexp => sign resolved_st_q => sign resolved_st_q" where
+  "assume_sign_st_for source_global b s =
+    bfilter_sign_st source_global b True s"
+
+definition assume_not_sign_st_for ::
+  "(vname => bool) => bexp => sign resolved_st_q => sign resolved_st_q" where
+  "assume_not_sign_st_for source_global b s =
+    bfilter_sign_st source_global b False s"
+
+definition sign_enter_st_for ::
+  "(vname => bool) => vname list => aexp list =>
+   sign resolved_st_q => sign resolved_st_q" where
+  "sign_enter_st_for source_global xs es s =
+    bind_formals_resolved_q source_global xs
+      (map (\<lambda>e. aval_sign e
+        (fun_of_resolved_st_q_for source_global s)) es)
+      (enter_frame_D_resolved_q STop s)"
+
+fun sign_tf_st_for ::
+  "(vname => bool) => edge_action =>
+   sign resolved_st_q => sign resolved_st_q" where
+    "sign_tf_st_for source_global EA_Nop s = s"
+  | "sign_tf_st_for source_global (EA_Assign x a) s =
+       update_resolved_st_q s (location_of source_global x)
+         (aval_sign a (fun_of_resolved_st_q_for source_global s))"
+  | "sign_tf_st_for source_global (EA_Assume b) s =
+       assume_sign_st_for source_global b s"
+  | "sign_tf_st_for source_global (EA_AssumeNot b) s =
+       assume_not_sign_st_for source_global b s"
+  | "sign_tf_st_for source_global (EA_Ret None p) s = s"
+  | "sign_tf_st_for source_global (EA_Ret (Some a) p) s =
+       update_resolved_st_q s (location_of source_global ret_var)
+         (aval_sign a (fun_of_resolved_st_q_for source_global s))"
+
+text \<open>The Nop/Assign executable-abstract correspondence facts, mirroring
+  \<open>ivl_tf_st_for_nop_agree\<close>/\<open>ivl_tf_st_for_assign_agree\<close> for the interval
+  domain: given only scoped input agreement (and, for a write, that the
+  written expression's value already agrees), the executable step agrees
+  with the abstract step at every location the scope covers.\<close>
+
+lemma sign_tf_st_for_nop_agree:
+  fixes s_exec :: "sign resolved_st_q" and s_abs :: "sign abs_state"
+  assumes agree: "\<And>location. location \<in> universe \<Longrightarrow>
+      lookup_resolved_st_q s_exec location = s_abs (location_vname location)"
+    and location_in: "location \<in> universe"
+  shows
+    "lookup_resolved_st_q (sign_tf_st_for gs EA_Nop s_exec) location =
+      apply_tf (sign_tf_for gs) EA_Nop s_abs (location_vname location)"
+  using agree[OF location_in] by simp
+
+lemma sign_tf_st_for_assign_agree:
+  fixes y :: vname and a :: aexp
+  assumes agree: "\<And>location. location \<in> universe \<Longrightarrow>
+      lookup_resolved_st_q s_exec location = s_abs (location_vname location)"
+    and val_agree: "aval_sign a (fun_of_resolved_st_q_for gs s_exec) = aval_sign a s_abs"
+    and location_in: "location \<in> universe"
+    and canonical: "location = location_of gs (location_vname location)"
+  shows
+    "lookup_resolved_st_q (sign_tf_st_for gs (EA_Assign y a) s_exec) location =
+      apply_tf (sign_tf_for gs) (EA_Assign y a) s_abs (location_vname location)"
+proof (cases "location_vname location = y")
+  case True
+  then have "location = location_of gs y" using canonical by simp
+  then show ?thesis using val_agree True by (simp add: sign_tf_for_def assign_sign_def)
+next
+  case False
+  have neq: "location \<noteq> location_of gs y"
+  proof
+    assume eq: "location = location_of gs y"
+    have "location_vname location = y" using eq by (simp add: location_of_def)
+    with False show False by simp
+  qed
+  show ?thesis
+    using agree[OF location_in] neq False by (simp add: sign_tf_for_def assign_sign_def)
+qed
+
+lemma sign_tf_st_for_ret_none_agree:
+  fixes s_exec :: "sign resolved_st_q" and s_abs :: "sign abs_state"
+  assumes agree: "\<And>location. location \<in> universe \<Longrightarrow>
+      lookup_resolved_st_q s_exec location = s_abs (location_vname location)"
+    and location_in: "location \<in> universe"
+  shows
+    "lookup_resolved_st_q (sign_tf_st_for gs (EA_Ret None p) s_exec) location =
+      apply_tf (sign_tf_for gs) (EA_Ret None p) s_abs (location_vname location)"
+  using sign_tf_st_for_nop_agree[OF agree location_in]
+  by (simp add: apply_tf_EA_Ret_None)
 
 end
 
